# Discrete math assignment 1

Q1 
1a  
use mathematical induction.  
First we prove $(\frac{3}{2})^{n-1}<f_n (n\ge 6)$ (lower bound)    

1. For $n = 6$ ,
$(\frac{3}{2})^5 = 7.59375 < f_6 = 8$  
1. Suppose $(\frac{3}{2})^{n-1}<f_n$ is true when $n = k (k\ge 6)$.  
2. When $n = k+1 (k\ge 6)$,  
$f_n = f_{k+1}=f_k+f_{k-1}>(\frac{3}{2})^{k-1} +(\frac{3}{2})^{k-2}=(\frac{3}{2})^{k-2}*(\frac{3}{2}+1)>(\frac{3}{2})^{k-2}*(\frac{9}{4})=(\frac{3}{2})^{k}$  

So  $(\frac{3}{2})^{n-1}<f_n (n\ge 6)$   (1)
****
Then we prove the upper bound  
1. For $n = 6$ ,
$f_6 = 8<(\frac{5}{3})^5 = 12.860$  

2. Suppose $f_n < (\frac{5}{3})^{n-1}$ is true when $n = k (k\ge 6)$.  
   
3. When $n = k+1 (k\ge 6)$,  
   $f_n = f_{k+1}=f_k+f_{k-1} < (\frac{5}{3})^{k-1} +(\frac{5}{3})^{k-2}=(\frac{5}{3})^{k-2}*(\frac{5}{3}+1)<(\frac{5}{3})^{k-2}*(\frac{25}{9})=(\frac{5}{3})^{k}$  

So  $f_n < (\frac{5}{3})^{n-1}(n\ge 6)$   (2)  

By (1) and (2),
$(\frac{3}{2})^{n-1}< f_n < (\frac{5}{3})^{n-1}(n\ge 6)$  

(b)   
A possible value of $c$ is $c = 30$, to prove this, we use mathematical induction.  
 

we first prove the lower bound:
1. when $n = 30$  
   $(\frac{8}{5})^{29} = 830767.50<fib_{30}=832040$   
2. Suppose $f_n > (\frac{8}{5})^{n-1}$ is true when $n = k (k \ge 30)$.
3. When $n = k+1 (k\ge 30)$,  
   $f_n = f_{k+1}=f_k+f_{k-1} > (\frac{8}{5})^{k-1} +(\frac{8}{5})^{k-2}=(\frac{8}{5})^{k-2}*(\frac{8}{5}+1)>(\frac{8}{5})^{k-2}*(\frac{64}{25})=(\frac{8}{5})^{k}$  

So $f_n > (\frac{8}{5})^{n-1}(n\ge 30)$   (1)   

Then we prove the upper bound:
1. when $n = 30$  
   $fib_{30}=832040<(\frac{13}{8})^{29} = 1302409.62$   
2. Suppose $f_n < (\frac{13}{8})^{n-1}$ is true when $n = k (k \ge 30)$.
3. When $n = k+1 (k\ge 30)$,  
   $f_n = f_{k+1}=f_k+f_{k-1} < (\frac{13}{8})^{k-1} +(\frac{13}{8})^{k-2}=(\frac{13}{8})^{k-2}*(\frac{13}{8}+1)<(\frac{13}{8})^{k-2}*(\frac{169}{64})=(\frac{13}{8})^{k}$  

So $f_n < (\frac{13}{8})^{n-1}(n\ge 30)$   (2)   

By (1) and (2),
$(\frac{8}{5})^{n-1}< f_n < (\frac{13}{8})^{n-1}(n\ge 30)$  


****
Q2  

c  

Every number in $N$ is divisible by 1.   

$x\in N \rightarrow x$ is divisible by 1 (There exists a number in $N$ that divides $x$)  
$A = (x+y|x \in N, y \in N) \subseteq N$  
So $n \in A \rightarrow P(x,y,z)$
Above establishes that ...   


****

Q3 
a  
To show that $n!$ is not $O(3^n)$, we use prove by contradiction.  

Suppose that there are constant pair $C$ and $k$ such that $n!\le C*3^n$ for all $n>k$, then their exists  constant $C \ge \frac{n!}{3^n} (n>k)$.  
However, $\lim_{n \to \infty}(\frac{n!}{3^n}) =+\infty$ (not converges to a constant). In other words, their is no such $C$ that is not less than all possible $\frac{n!}{3^n}(n>k)$), which contradict with our premise.  
This contradiction shows that $n!$ is not $O(3^n)$




b  
Note that $n^2>n$ and $n^2>1$ when $n>1$  
$3n^2+4n+5 <3n^2+4n^2+5n^2=12n^2(n>1)$
Thus, there exists constants $C = 12, k=1$,  
$|3n^2+4n+5|\le C|n^2|$ whenever $n>k$.  
so, $3n^2+4n+5$ is $O(n^2)$


c  
The algorithm is based on Horners' rule (秦九韶算法).  

   Evaluate (Array A[0..n], Integer x)  
   1. Integer result$\leftarrow$ A[n]
   2. for Integer i $\leftarrow$ n to 1
   3. result = result * x + a[i]
   4. return result

Analysis of the `Evaluate`
- Line 1: $O(1)$  
- Line 2: n times = $O(n)$  
- Line 3: n times = $O(n)$  
- Line 4: $O(1)$  
  
Worst-case running time = $O(1)+O(n)+O(n)+O(1) = O(n)$
****



Q4 
a  
$(A-B) = ({x|x\in A \wedge x \notin B})$  
$(A-B)-C = ({y| y \in ({x|x\in A \wedge x \notin B}) \wedge y \notin B}) = ({x|x \in A \wedge x \notin B \wedge x \notin C})$

$(A-C) = ({x|x\in A \wedge x \notin C})$  
Thus,  
$(x \in (A-B)-C) \to (x \in (A-C)) \Rightarrow (A-B)-C\subseteq(A-C)$  
This concludes the proof

Q4 b  
??  
singularity is a partition on Set $N$
So, or every x in $N$, it is either odd or even.
x can be represented either as $2n+1$ or $2n (n \in N)$

(1)
- if x is odd, then x+x = 4n+2, 4n+2 is even 
- if x is even, then x+x = 4n, 4n is even.

So for all $x \in N,(x,x)\in R$, R is reflexive.  
(2)   
integer addition is commutative,so $x+y = y+x$   
For all $(x,y) \in R$, $(y,x) \in R$  
Thus $R$ is symmetric.  
(3)  
consider the case (1,3) 1+3 is even so $(1,3) \in R$.

also we have 3+1 is even so $(3,1) \in R$

There exists pairs $(x,y) \in R$ and $(y,x) \in R$ but $(x,y) Ne (y,x)$  
Thus, R is not antisymmetric.  
(4)  
2n+2n+1 = 4n+1, so adding an odd and a even will result in an odd.  
So, if $if (x,y) \in R$, x and y must be either two odd numbers or two even numbers.  

if $(a,b)\in R, (b,c) \in R$, $a$ and $b$, $b$ and $c$ must be either two odd numbers or two even numbers. Then they are either all odd or all even.

- if they are odd, then a+c = 4n+2, 4n+2 is even 
- if they even, then a+c = 4n, 4n is even.

Thus, for all $(a,b) \in R$and $(a,c) \in R$, also $(a,c) \in R$.  $R$ is transitive.
